concurrency/juicy/resource_decay_lemmas.v
@@ -6,7 +6,7 @@ Require Import VST.veric.aging_lemmas.
 Require Import VST.veric.juicy_mem.
 Require Import VST.veric.juicy_mem_lemmas.
 Require Import VST.veric.compcert_rmaps.
-Require Import VST.veric.Clight_new.
+Require Import VST.veric.Clight_core.
 Require Import VST.veric.semax.
 Require Import VST.veric.semax_ext.
 Require Import VST.veric.juicy_extspec.
