concurrency/juicy/semax_safety_makelock.v
@@ -18,8 +18,8 @@ Require Import VST.veric.juicy_mem.
 Require Import VST.veric.juicy_mem_lemmas.
 Require Import VST.veric.semax_prog.
 Require Import VST.veric.compcert_rmaps.
-Require Import VST.veric.Clight_new.
-Require Import VST.veric.Clightnew_coop.
+Require Import VST.veric.Clight_core.
+Require Import VST.concurrency.common.Clightcore_coop.
 Require Import VST.veric.semax.
 Require Import VST.veric.semax_ext.
 Require Import VST.veric.juicy_extspec.
@@ -114,7 +114,6 @@ Proof.
     as [ | ?????? bad | n0 z c m0 e args0 x at_ex Pre SafePost | ????? bad ].
   apply (corestep_not_at_external (juicy_core_sem _)) in bad. elimtype False; subst; clear - bad atex.
    simpl in bad. unfold cl_at_external in *; simpl in *. rewrite atex in bad; inv bad.
-  2: inversion bad.
   subst.
   simpl in at_ex.
   unfold cl_at_external in atex, at_ex.
