veric/juicy_extspec.v
@@ -33,14 +33,14 @@ Definition void_spec T : external_specification juicy_mem external_function T :=
       (fun ef => False)
       (fun ef Hef ge tys vl m z => False)
       (fun ef Hef ge ty vl m z => False)
-      (fun rv m z => False).
+      (fun rv m z => True).
 
 Definition ok_void_spec (T : Type) : OracleKind.
  refine (Build_OracleKind T (Build_juicy_ext_spec _ (void_spec T) _ _ _)).
 Proof.
   simpl; intros; contradiction.
   simpl; intros; contradiction.
-  simpl; intros; intros ? ? ? ?; contradiction.
+  simpl; intros; intros ? ? ? ?; auto.
 Defined.
 
 Definition j_initial_core {C} (csem: @CoreSemantics C mem)
